PrimitiveFacts.v
@@ -1,0 +1,285 @@
+Require Import VST.floyd.functional_base.
+Require Import Poly.
+Require Import PolyMod.
+Require Import Coq.Logic.FinFun.
+Require Import Helper.
+Require Import InjectiveSurjective.
+Import WPoly.
+
+(** * Working with Primitive Polynomials and Primitive Elements*)
+
+Section Primitive.
+
+Variable f : poly.
+Variable Hnontrivial: deg f > 0.
+Variable Hprim: primitive f.
+
+(*we want to prove that x is a primitive element of GF(2)/(f) - ie, for any nonzero
+  poly p with degree smaller than deg f,
+  there is some 0 <= i < 2^(deg f) - 1 such that (x^i = p) mod f*)
+
+Definition bounded_int (u: nat) : Type := {z : Z | (0 <= z < Z.of_nat u) }.
+
+(*Prove that bounded ints are finite*)
+Definition all_bounded_ints_non_dep u : list Z :=
+  map (fun x => Z.of_nat x) (seq 0 u).
+
+Lemma all_bounded_ints_non_dep_spec: forall u z,
+  In z (all_bounded_ints_non_dep u) <-> (0 <= z < Z.of_nat u).
+Proof.
+  intros. unfold all_bounded_ints_non_dep. rewrite in_map_iff.  split; intros.
+  - destruct H. destruct H. rewrite in_seq in H0. lia.
+  - exists (Z.to_nat z). split. lia. rewrite in_seq. lia.
+Qed. 
+
+Lemma all_bounded_ints_non_dep_spec': forall u z,
+  In z (all_bounded_ints_non_dep u) -> (0 <= z < Z.of_nat u).
+Proof.
+  apply all_bounded_ints_non_dep_spec.
+Qed.
+
+Lemma all_bounded_ints_nodup: forall u, NoDup (all_bounded_ints_non_dep u).
+Proof.
+  intros. unfold all_bounded_ints_non_dep. apply Injective_map_NoDup.
+  unfold Injective. intros. lia. apply seq_NoDup.
+Qed.
+
+Definition all_bounded_ints u : list (bounded_int u) :=
+  exist_list _ (all_bounded_ints_non_dep u) (all_bounded_ints_non_dep_spec' u).
+
+Lemma all_bounded_ints_spec: forall u (b: bounded_int u),
+  In b (all_bounded_ints u).
+Proof.
+  intros. destruct b. unfold all_bounded_ints. apply exist_list_in.
+  simpl. apply all_bounded_ints_non_dep_spec. assumption.
+Qed.
+
+Lemma all_bounded_ints_length: forall u, length (all_bounded_ints u) = u.
+Proof.
+  intros. unfold all_bounded_ints. epose proof exist_list_length ((fun z : Z => 0 <= z < Z.of_nat u)).
+  rewrite H. unfold all_bounded_ints_non_dep. rewrite map_length. apply seq_length.
+Qed.
+
+(*The range of our function: nonzero qpolys*)
+(*ugh the nested dependent type is not very nice, maybe there is a better way*)
+Definition nonzero_qpoly := {q: qpoly f | proj1_sig q <> zero}.
+
+Lemma in_leq_degree_nonzero: forall x,
+  In x (polys_leq_degree_nonzero (Z.to_nat (deg f) - 1)) -> deg x < deg f.
+Proof.
+  intros. apply polys_leq_degree_nonzero_spec in H. lia.
+Qed.
+
+Definition list_of_qpoly_nonzero' : list (qpoly f) := exist_list (fun x => deg x < deg f) 
+  (polys_leq_degree_nonzero (Z.to_nat (deg f) - 1)) in_leq_degree_nonzero.
+
+Lemma in_leq_degree_nonzero_nonzero: forall x, In x (list_of_qpoly_nonzero') ->
+  proj1_sig x <> zero.
+Proof.
+  intros. unfold list_of_qpoly_nonzero' in H. rewrite (exist_list_in (fun x : poly => deg x < deg f))  in H.
+  apply polys_leq_degree_nonzero_spec in H. destruct H. assumption.
+Qed.
+
+Definition all_nonzero_qpolys: list (nonzero_qpoly) :=
+  exist_list _ list_of_qpoly_nonzero' (in_leq_degree_nonzero_nonzero).
+
+Lemma all_nonzero_qpolys_in: forall (q: nonzero_qpoly),
+  In q all_nonzero_qpolys.
+Proof.
+  intros. unfold all_nonzero_qpolys. rewrite (exist_list_in (fun x : qpoly f => proj1_sig x <> zero) ).
+  unfold list_of_qpoly_nonzero'. rewrite (exist_list_in  (fun x : poly => deg x < deg f)).
+  apply polys_leq_degree_nonzero_spec. destruct q. simpl. split. assumption.
+  destruct x. simpl. lia.
+Qed.
+
+Definition field_size := (2 ^ (Z.to_nat (deg f)) - 1)%nat.
+
+Lemma all_nonzero_qpolys_length: length (all_nonzero_qpolys) = field_size.
+Proof.
+  unfold field_size. unfold all_nonzero_qpolys. rewrite (exist_list_length (fun x : qpoly f => proj1_sig x <> zero)).
+  unfold list_of_qpoly_nonzero'. rewrite (exist_list_length (fun x : poly => deg x < deg f)).
+  rewrite polys_leq_degree_nonzero_length.
+  assert ((Z.to_nat (deg f) - 1 + 1)%nat = Z.to_nat (deg f)) by lia. rewrite H. reflexivity.
+Qed.
+
+Lemma all_nonzero_qpolys_NoDups: NoDup (all_nonzero_qpolys).
+Proof.
+  unfold all_nonzero_qpolys. rewrite (exist_list_NoDup (fun x : qpoly f => proj1_sig x <> zero)).
+  unfold list_of_qpoly_nonzero'. rewrite (exist_list_NoDup (fun x : poly => deg x < deg f)).
+  apply polys_leq_degree_nonzero_NoDup.
+Qed.
+
+Lemma bounded_int_listing: forall u, Listing (all_bounded_ints u).
+Proof.
+  intros. unfold Listing. split. unfold all_bounded_ints.
+  rewrite (exist_list_NoDup  (fun z : Z => 0 <= z < Z.of_nat u)). apply all_bounded_ints_nodup.
+  unfold Full. apply all_bounded_ints_spec.
+Qed.
+
+Lemma nonzero_qpoly_listing: Listing (all_nonzero_qpolys).
+Proof.
+  unfold Listing. split. apply all_nonzero_qpolys_NoDups. unfold Full. apply all_nonzero_qpolys_in.
+Qed.
+
+(*We now define the map i -> (x^i %f) for 0 <= i < 2^(deg f) - 1 and show that it is injective. Since boundedInts
+  are finite, it is surjective as well*)
+
+
+
+Definition primitive_map' (b: bounded_int field_size) : qpoly f :=
+  exist _ (monomial (Z.to_nat (proj1_sig b)) %~ f) (pmod_lt_deg f Hnontrivial _).
+
+(*TODO move*)
+Lemma monomial_exp_law: forall a b,
+  monomial a *~ monomial b = monomial (a + b).
+Proof.
+  intros. rewrite <- shift_monomial. unfold monomial. unfold shift. 
+  destruct (destruct_poly (exist PolyDefs.P.wf_poly (PolyDefs.P.monomial b) (PolyDefs.P.wf_monomial b))).
+  - unfold zero in e. inversion e. exfalso. eapply PolyDefs.P.monomial_not_0. apply H0.
+  - exist_eq. simpl. unfold PolyDefs.P.shift.
+    unfold PolyDefs.P.monomial. if_tac.
+    + subst. if_tac. assert (a = 0%nat) by lia. subst. simpl. reflexivity. unfold PolyDefs.P.shift.
+      replace (a + 0)%nat with (a) by lia. reflexivity.
+    + if_tac. lia. unfold PolyDefs.P.shift.
+      rewrite <- list_repeat_app. rewrite app_assoc. reflexivity.
+Qed.
+
+(*move this too*)
+Definition x : poly := monomial 1.
+
+Lemma deg_x: deg x = 1%Z.
+Proof.
+  intros. unfold x. unfold monomial. unfold deg. simpl. reflexivity.
+Qed.
+
+Lemma monomial_expand: forall n,
+  monomial (S(n)) = x *~ monomial n.
+Proof.
+  intros. replace (S(n)) with (n+1)%nat by lia. rewrite <- monomial_exp_law.
+  unfold x. apply poly_mult_comm.
+Qed.
+
+Lemma divides_x: forall (g: poly),
+  deg g > 0 ->
+  g |~ x <-> g = x.
+Proof.
+  intros.
+  - unfold divides. split; intros.
+    + destruct H0. assert (deg (g *~ x0) = deg x) by (rewrite H0; reflexivity).
+      destruct (destruct_poly x0). subst.
+      rewrite poly_mult_0_r in H0. inversion H0.
+      rewrite poly_mult_deg in H1. rewrite deg_x in H1.
+      rewrite <- deg_nonzero in n.
+      assert (deg g = 1%Z /\ deg x0 = 0%Z) by lia. destruct H2.
+      symmetry in H3. rewrite deg_one in H3. subst. rewrite poly_mult_1_r in H0.
+      assumption. apply f_nonzero. assumption. assumption.
+    + subst. exists one. apply poly_mult_1_r.
+Qed.
+
+(*maybe move also*)
+(*x is an annoying special case - x is irreducible but no other powers of x are *)
+Lemma irred_doesnt_divide_monomial: forall (g: poly) (n: nat),
+  deg g > 0 ->
+  irreducible g ->
+  g <> x ->
+  ~ (g |~ (monomial n)).
+Proof.
+  intros. induction n.
+  - rewrite monomial_0. intro. unfold divides in H2. destruct H2.
+    apply poly_mult_eq_one in H2. destruct H2. subst.
+    assert (0%Z = deg one) by (rewrite deg_one; reflexivity). lia.
+  - rewrite monomial_expand. intro. 
+    apply irreducible_is_prime in H0. unfold prime in H0. apply H0 in H2.
+    destruct H2. 
+    + apply divides_x in H2. subst. contradiction. assumption.
+    + contradiction.
+Qed.
+
+
+Lemma primitive_map'_nonzero: forall b,
+  proj1_sig (primitive_map' b) <> zero.
+Proof.
+  intros. unfold primitive_map'. simpl. intro.
+  destruct b; simpl in H.
+  assert (f |~ (monomial (Z.to_nat x0))). rewrite divides_pmod_iff.
+  unfold divides_pmod. apply H. left. apply f_nonzero. assumption. 
+  destruct (poly_eq_dec f x).
+  - unfold field_size in a. rewrite e in a. rewrite deg_x in a. simpl in a.
+    assert (x0 = 0%Z) by lia. rewrite H1 in H0. simpl in H0. 
+    rewrite monomial_0 in H0. unfold divides in H0.
+    subst. destruct H0. apply poly_mult_eq_one in H0.
+    destruct H0. subst. rewrite H0 in Hnontrivial.
+    assert (0%Z = deg one) by (apply deg_one; reflexivity). lia.
+  - apply (irred_doesnt_divide_monomial f (Z.to_nat x0)); try assumption.
+    unfold primitive in Hprim. apply Hprim.
+Qed.
+
+Definition primitive_map (b: bounded_int field_size) : nonzero_qpoly :=
+  exist _ (primitive_map' b) (primitive_map'_nonzero b). 
+
+Lemma primitive_map_injective: Injective primitive_map.
+Proof.
+  unfold Injective. intros. unfold primitive_map in H. inversion H. clear H.
+  destruct x0; destruct y; simpl in H1. exist_eq.
+  rewrite pmod_cancel in H1; try assumption.
+  (*special case - if f is x - then GF(2)/(x) = GF(2) - only 2 elements to deal with - only nontrivial elt is 1*)
+  destruct (poly_eq_dec f x).
+  - rewrite e in H1. assert (field_size = 1%nat). unfold field_size.
+    rewrite e. rewrite deg_x. simpl. reflexivity. rewrite H in a. simpl in a. rewrite H in a0.
+    simpl in a0. lia. 
+  -
+  (*2 cases are the same, so we abstract in an assertion*)
+  (*Proof idea: if x^i = x^j mod f, wlog assume i <= j. Then x^ix^(j-i) - x^i = 0 %f, so
+    x^i(x^(j-i) - 1) = 0% f. Since f is irreducible, x^i = 0 % f or x^(j-i) -1 = 0 % f.
+    In the first case, x^i = q * f, so f has the factor x (x itself is a special case),
+    in the second case, this contradicts the definition of a primitive poly, since j - i < 2 ^ deg f - 1*)
+  assert (forall y y', (0 <= y < Z.of_nat field_size) -> (0 <= y' < Z.of_nat field_size) ->
+  (monomial (Z.to_nat y) +~ monomial (Z.to_nat y')) %~ f = zero -> y <= y' -> y = y'). {
+  intros. assert ((Z.to_nat y') = (Z.to_nat y +  Z.to_nat (y' - y))%nat) by lia.
+  rewrite H4 in H2. rewrite <- monomial_exp_law in H2.
+  rewrite <- (poly_mult_1_r (monomial (Z.to_nat y))) in H2 at 1.
+  rewrite <- poly_mult_distr_l in H2.
+  apply irreducible_integral_domain in H2; try assumption.
+  destruct H2.
+  - unfold pmod in H2. destruct (poly_div (monomial (Z.to_nat y)) f ) as [q r] eqn : P.
+    simpl in H2. subst. rewrite poly_div_correct in P; try assumption.
+    destruct P. rewrite poly_add_0_r in H2.
+    assert (f |~ monomial (Z.to_nat y)). unfold divides. exists q. rewrite H2. apply poly_mult_comm.
+    exfalso. apply (irred_doesnt_divide_monomial f (Z.to_nat y)); try assumption. unfold primitive in Hprim.
+    apply Hprim. apply f_nonzero. assumption.
+  - unfold primitive in Hprim. 
+    assert (f |~ nth_minus_one (Z.to_nat (y' - y))). unfold nth_minus_one.
+    rewrite poly_add_comm. rewrite divides_pmod_iff. unfold divides_pmod. apply H2. left.
+    apply f_nonzero; assumption. destruct Hprim. destruct H7. destruct H8.
+    apply H9 in H5. 
+    destruct H5. lia. unfold field_size in H. unfold field_size in H0. lia.
+  - unfold primitive in Hprim. apply Hprim. }
+  assert (x0 <= x1 \/ x0 > x1) by lia.
+  destruct H0. apply H; try assumption. 
+  symmetry. apply H; try assumption; try lia. rewrite poly_add_comm. apply H1.
+Qed.
+
+Lemma primitive_map_surjective: Surjective primitive_map.
+Proof.
+  eapply injective_surjective.
+  apply (bounded_int_listing field_size). 
+  apply nonzero_qpoly_listing.
+  rewrite all_nonzero_qpolys_length.
+  rewrite all_bounded_ints_length. lia. 
+  apply primitive_map_injective.
+Qed.
+
+Lemma primitive_power_exists: forall (q: qpoly f),
+  (proj1_sig q <> zero) ->
+  exists (n: Z), (0 <= n < Z.of_nat field_size)%Z /\ monomial (Z.to_nat n) %~ f = (proj1_sig q).
+Proof.
+  intros. pose proof (primitive_map_surjective). unfold Surjective in H0.
+  remember (exist (fun x => proj1_sig x <> zero) q H) as q'.
+  specialize (H0 q'). destruct H0. destruct x0. exists x0. split. assumption.
+  rewrite Heqq' in H0. unfold primitive_map in H0. inversion H0.
+  destruct q. unfold primitive_map' in H2. inversion H2.
+  simpl. reflexivity.
+Qed.
+
+(*TODO: function that finds power of primitive element - then start C code*)
+End Primitive.
